Flapjack/Tests.lean
@@ -72,6 +72,7 @@ import Flapjack.Test.RuntimeLinking
 import Flapjack.Test.CallEntry
 import Flapjack.RiscV.CorrectnessSpill
 import Flapjack.Test.SpillRelation
+import Flapjack.Test.LocationMoveRelation
 import Flapjack.RiscV.CorrectnessBinarySpill
 import Flapjack.Test.BinarySpillRelation
 import Flapjack.RiscV.CorrectnessShiftSpill
